[rpc] Remove counters from specifications.

rpc/proofs.v
@@ -27,28 +27,24 @@ Implicit Types n : nat.
 Implicit Types γ : gname.
 Implicit Types v : val.
 
-Lemma wp_connect P N c kI kR n :
+Lemma wp_connect P N c kI kR :
   channel c -∗
   cryptis_ctx -∗
   ctx N -∗
   sign_key kI -∗
   public (TKey Open kR) -∗
-  {{{ client_disconnected N kI kR n ∗ (Conn.failure kI kR ∨ P) }}}
+  {{{ Conn.failure kI kR ∨ P }}}
     Impl.connect N c kI (TKey Open kR)
   {{{ cs, RET (repr cs);
-      client_connected N kI kR cs n ∗
+      client_connected kI kR cs ∗
       (compromised_session Init cs ∨ P) }}}.
 Proof.
-iIntros "#? #? #? #? #? % !> (clock & P) post".
-iPoseProof (or_sep1 with "clock P") as "P".
+iIntros "#? #? #? #? #? % !> P post".
 wp_lam; wp_pures.
 iPoseProof (Props.ctx_conn_ctx with "[//]") as "?".
 iApply wp_fupd.
 wp_apply (Conn.wp_connect with "[//] [//] [//] [//] [//] P").
 iIntros "%cs (connected & P & rel & token)".
-iMod (term_meta_set (isoN.@"conn".@"beg") n with "token")
-  as "#meta"; first solve_ndisj.
-iDestruct (or_sep2 with "P") as "[clock P]".
 iApply "post". by iFrame.
 Qed.
 
@@ -66,59 +62,44 @@ wp_lam. iApply Conn.wp_listen => //.
 by iApply Props.ctx_conn_ctx.
 Qed.
 
-Lemma wp_confirm P N c skA skB ga n :
+Lemma wp_confirm P N c skA skB ga :
   channel c -∗
   cryptis_ctx -∗
   ctx N -∗
   {{{ public ga ∗ public (TKey Open skA) ∗ sign_key skB ∗
-      server_disconnected N skA skB n ∗
       (Conn.failure skA skB ∨ P) }}}
     confirm N c skB (ga, TKey Open skA)%V
   {{{ cs, RET (repr cs);
-      server_connected N skA skB cs n ∗
+      server_connected skA skB cs ∗
       (compromised_session Resp cs ∨ P) }}}.
 Proof.
-iIntros "#? #ctx #? !> %Φ (#p_ga & #p_vkA & #sign_skB & dis & P) post".
-iPoseProof (or_sep1 with "dis P") as "dis".
+iIntros "#? #ctx #? !> %Φ (#p_ga & #p_vkA & #sign_skB & P) post".
 wp_lam; wp_pures.
 iPoseProof (Props.ctx_conn_ctx with "[//]") as "?".
 iApply wp_fupd.
-wp_apply (Conn.wp_confirm (server_clock N skA skB n ∗ P)
-           with "[//] [//] [//] [$dis]").
+wp_apply (Conn.wp_confirm P with "[//] [//] [//] [$P]").
 { by eauto. }
 iIntros "%cs (conn & dis & rel & token)".
-iMod (term_meta_set (isoN.@"conn".@"beg") n with "token")
-  as "#meta"; first solve_ndisj.
-iDestruct (or_sep2 with "dis") as "[dis P]".
 iApply "post". by iFrame.
 Qed.
 
-Lemma wp_call N s φ ψ kI kR c cs n (ts : list term) :
+Lemma wp_call N s φ ψ kI kR c cs (ts : list term) :
   {{{ channel c ∗ cryptis_ctx ∗ ctx N ∗
       ([∗ list] t ∈ ts, public t) ∗
       rpc_pred N s φ ψ ∗
-      client_connected N kI kR cs n ∗
-      (compromised_session Init cs ∨ φ kI kR cs n ts) }}}
+      client_connected kI kR cs ∗
+      (compromised_session Init cs ∨ φ kI kR cs ts) }}}
     call N s c (repr cs) (repr ts)
   {{{ ts', RET (repr ts');
-      client_connected N kI kR cs (S n) ∗
-      (compromised_session Init cs ∨ ψ kI kR cs n ts') ∗
+      client_connected kI kR cs ∗
+      (compromised_session Init cs ∨ ψ kI kR cs ts') ∗
       ([∗ list] t ∈ ts', public t) }}}.
 Proof.
 iIntros "%Φ (#? & #? & #? & #p_ts & #(? & ?) & conn & inv) post".
-iDestruct "conn" as "(conn & rel & clock)".
+iDestruct "conn" as "(conn & rel)".
 wp_lam. wp_pure _ credit:"c". wp_pures.
-iAssert (|==>
-  compromised_session Init cs ∨
-  client_clock N kI kR (S n) ∗ tick N kI kR n)%I
-  with "[clock]" as ">clock".
-{ iDestruct "clock" as "[?|[clock tock]]"; eauto.
-  iMod (tock_tick with "clock tock") as "(_ & ?)"; eauto. }
-rewrite or_sep2. iDestruct "clock" as "[clock tick]".
-wp_apply (Conn.wp_write with "[//] [] [] [$conn tick inv]"); eauto.
-{ iDestruct "inv" as "[(_ & ? & _)|inv]"; first by eauto.
-  iDestruct "tick" as "[(_ & ? & _)|tick]"; first by eauto.
-  iRight. iExists n. by iFrame. }
+wp_apply (Conn.wp_write with "[//] [] [] [$conn inv]"); eauto.
+{ iDestruct "inv" as "[(_ & ? & _)|inv]"; first by eauto. by iRight. }
 iIntros "conn". wp_pures. iApply wp_fupd.
 wp_apply (Conn.wp_read with "[//] [] [$conn]"); eauto.
 iIntros "%ts' (conn & p_ts' & inv)".
@@ -126,28 +107,18 @@ iApply "post". iDestruct "inv" as "[#inv|inv]".
 { iAssert (public (TKey Open (si_key cs))) as "?".
   { iApply public_TKey. by eauto. }
   iPoseProof (Conn.connected_public_key with "conn rel [//]") as "#>?".
-  iFrame. iModIntro. iSplitR; eauto. }
-iDestruct "inv" as "(%m & tock & inv)".
-iFrame. iDestruct "clock" as "[#?|clock]".
-{ iModIntro. iSplitL; eauto. }
-iPoseProof (client_clock_tock with "clock tock") as "%e".
-case: e => <-.
-iModIntro. iSplitR "inv"; eauto.
-iRight. iFrame.
+  iFrame. iModIntro. by eauto. }
+by iFrame.
 Qed.
 
-Definition wf_handler Φ kI kR cs N h : iProp :=
+Definition wf_handler Φ kI kR cs h : iProp :=
   Conn.wf_handler
-    (∃ n,
-        release_token (si_resp_share cs) ∗ Φ n ∗
-        (compromised_session Resp cs ∨ server_clock N kI kR n))%I
-    (λ r, ∃ n,
-      ⌜r = #true⌝ ∗ Φ n ∗
+    (release_token (si_resp_share cs) ∗ Φ)%I
+    (λ r,
+      ⌜r = #true⌝ ∗ Φ ∗
       Conn.connected kI kR Resp cs ∗
-      (compromised_session Resp cs ∨ server_clock N kI kR n) ∗
       release_token (si_resp_share cs) ∨
-      ⌜r = #false⌝ ∗ Φ n ∗
-      (compromised_session Resp cs ∨ server_clock N kI kR n) ∗
+      ⌜r = #false⌝ ∗ Φ ∗
       public (si_key cs))%I
     kI kR Resp cs h.
 
@@ -156,21 +127,21 @@ Lemma wp_handle Φ N s φ₁ φ₂ kI kR c cs (f : val) :
     channel c ∗
     rpc_pred N s φ₁ φ₂ ∗
     ctx N ∗
-    □ (∀ n (ts : list term),
+    □ (∀ (ts : list term),
       {{{ ▷ ([∗ list] t ∈ ts, public t) ∗
-          ▷ (compromised_session Resp cs ∨ φ₁ kI kR cs n ts) ∗
-          Φ n }}}
+          ▷ (compromised_session Resp cs ∨ φ₁ kI kR cs ts) ∗
+          Φ }}}
         f (repr ts)
       {{{ ts', RET (repr ts');
           match ts' with
           | Some ts' => ([∗ list] t ∈ ts', public t) ∗
-                        (compromised_session Resp cs ∨ φ₂ kI kR cs n ts')
+                        (compromised_session Resp cs ∨ φ₂ kI kR cs ts')
           | None => True
           end ∗
-          Φ (S n) }}})
+          Φ }}})
   }}}
     handle N s c f
-  {{{ h, RET (repr h); wf_handler Φ kI kR cs N h }}}.
+  {{{ h, RET (repr h); wf_handler Φ kI kR cs h }}}.
 Proof.
 iIntros "%Ψ (#chan_c & (#? & #?) & #ctx & #wp_f) post".
 iPoseProof (ctx_error with "[//]") as "#?".
@@ -178,29 +149,16 @@ wp_lam; wp_pures.
 iApply Conn.wp_handle; last by eauto.
 iSplit => //. clear Ψ.
 iIntros "!> %ts !> %Ψ (conn & I & #p_ts & inv_ts) post".
-iDestruct "I" as "(%n & rel & I & clock)". wp_pures.
+iDestruct "I" as "(rel & I)". wp_pures.
 iAssert (Conn.connected kI kR Resp cs ∗
          release_token (si_resp_share cs) ∗
-         ◇ (compromised_session Resp cs ∨ call_pred N φ₁ kI kR cs ts))%I
+         ◇ (compromised_session Resp cs ∨ φ₁ kI kR cs ts))%I
   with "[conn rel inv_ts]" as "(conn & rel & >inv_ts)".
 { iDestruct "inv_ts" as "[#fail|inv_ts]"; last by iFrame.
   iAssert (public (TKey Open (si_key cs))) as "?".
   { iApply public_TKey. by eauto. }
   iPoseProof (Conn.connected_public_key with "conn rel [//]") as "#H".
   iFrame. iMod "H" as "?". by eauto. }
-iAssert (|==>
-           compromised_session Resp cs ∨
-           server_clock N kI kR (S n) ∗
-           φ₁ kI kR cs n ts ∗
-           tock N kI kR (S n))%I
-    with "[clock inv_ts]" as ">H".
-{ iDestruct "clock" as "[?|clockS]"; first by eauto.
-  iDestruct "inv_ts" as "[?|inv_ts]"; first by eauto.
-  iDestruct "inv_ts" as "(%m & clockC & inv)".
-  iMod (tick_tock with "clockS clockC") as "(-> & clockS & clockC)".
-  iModIntro. iRight. by iFrame. }
-iPoseProof (or_sep2 with "H") as "[clockS H]".
-iPoseProof (or_sep2 with "H") as "[inv clockC]".
 wp_apply ("wp_f" with "[$]"). iIntros "%ts' (inv_ts' & inv)".
 case: ts' => [ts'|]; wp_pures; last first.
 { wp_list.
@@ -208,20 +166,19 @@ case: ts' => [ts'|]; wp_pures; last first.
   { by rewrite /= public_TInt. }
   { by iRight. }
   iIntros "conn". wp_pures.
-  iApply "post". iModIntro. iExists (S n). iLeft. by iFrame. }
+  iApply "post". iModIntro. iLeft. by iFrame. }
 iDestruct "inv_ts'" as "(#p_ts' & inv_ts')".
-wp_apply (Conn.wp_write with "[//] [] [] [inv_ts' clockC $conn]") => //.
+wp_apply (Conn.wp_write with "[//] [] [] [inv_ts' $conn]") => //.
 { iDestruct "inv_ts'" as "[(_ & ? & _)|inv_ts']"; first by eauto.
-  iDestruct "clockC" as "[(_ & ? & _)|clockC]"; first by eauto.
-  iRight. iExists n. iFrame. }
+  by eauto. }
 iIntros "conn". wp_pures. iApply "post". iModIntro.
-iExists (S n). iLeft. by iFrame.
+iLeft. by iFrame.
 Qed.
 
 Lemma wp_handle_close Φ N c kI kR cs :
   {{{ channel c ∗ ctx N }}}
     handle_close N c
-  {{{ h, RET (repr h); wf_handler Φ kI kR cs N h }}}.
+  {{{ h, RET (repr h); wf_handler Φ kI kR cs h }}}.
 Proof.
 iIntros "%Ψ (#chan_c & #ctx) post". wp_lam; wp_pures.
 wp_apply Conn.wp_handle; last by eauto. clear Ψ.
@@ -229,7 +186,7 @@ iPoseProof (ctx_close with "ctx") as "#?".
 iPoseProof (ctx_ack_close with "ctx") as "#?".
 iSplit => //.
 iIntros "!> %ts !> %Ψ (conn & inv & #p_ts & #inv_ts) post".
-iDestruct "inv" as "(%n & rel & inv & clockS)". wp_pures.
+iDestruct "inv" as "(rel & inv)". wp_pures.
 iMod (release with "rel") as "#relS".
 iPoseProof (Conn.connected_released_session with "conn") as "#s_k".
 iAssert (|==> public (si_key cs))%I as ">#p_k".
@@ -241,47 +198,44 @@ wp_apply (Conn.wp_write with "[//] [] [] [$conn]") => //.
 - by iLeft.
 iIntros "conn". wp_pures. wp_apply (Conn.wp_free with "[$conn]").
 iIntros "_". wp_pures. iApply "post".
-iExists n. iModIntro. iFrame. iRight. by eauto.
+iModIntro. iFrame. iRight. by eauto.
 Qed.
 
-Lemma wp_server Φ N kI kR c cs n handlers :
+Lemma wp_server Φ N kI kR c cs handlers :
   {{{ channel c ∗ ctx N ∗
-      server_connected N kI kR cs n ∗ Φ n ∗
-      [∗ list] h ∈ handlers, wf_handler Φ kI kR cs N h }}}
+      server_connected kI kR cs ∗ Φ ∗
+      [∗ list] h ∈ handlers, wf_handler Φ kI kR cs h }}}
     server N c (repr cs) (repr handlers)
-  {{{ RET #(); ∃ n', server_disconnected N kI kR n' ∗
-                     public (si_key cs) ∗ Φ n' }}}.
+  {{{ RET #(); public (si_key cs) ∗ Φ }}}.
 Proof.
-iLöb as "IH" forall (n).
+iLöb as "IH".
 iIntros "%Ψ (#chan_c & #ctx & conn & inv & #handlers) post".
-iDestruct "conn" as "(conn & rel & clockS)".
+iDestruct "conn" as "(conn & rel)".
 iPoseProof (Conn.connected_keyE with "conn") as "#(-> & -> & _)".
 wp_rec. wp_pures. wp_apply (wp_handle_close Φ N _ _ _ cs); eauto.
 iIntros "%hc #wp_hc". wp_list.
-iAssert ([∗ list] h ∈ (hc :: handlers), wf_handler Φ _ _ cs N h)%I
+iAssert ([∗ list] h ∈ (hc :: handlers), wf_handler Φ _ _ cs h)%I
   as "#wp".
 { rewrite /=; iSplit => //. eauto. }
 iClear "wp_hc". wp_bind (Conn.select _ _ _).
-iApply (wp_wand with "[inv conn rel clockS]").
-{ wp_apply (Conn.wp_select with "chan_c wp [$conn $rel $inv $clockS]"). }
-iIntros "%res (%n' & Hres)".
+iApply (wp_wand with "[inv conn rel]").
+{ wp_apply (Conn.wp_select with "chan_c wp [$conn $rel $inv]"). }
+iIntros "%res Hres".
 iDestruct "Hres" as "[(-> & Hres)|(-> & Hres)]".
-- iDestruct "Hres" as "(inv & conn & clockS & rel)". wp_pures.
-  wp_apply ("IH" with "[$inv $clockS $rel $conn]") => //.
+- iDestruct "Hres" as "(inv & conn & rel)". wp_pures.
+  wp_apply ("IH" with "[$inv $rel $conn]") => //.
   by do !iSplit => //.
-- iDestruct "Hres" as "(inv & clockS & rel)". wp_pures.
-  iApply "post". iExists n'. iFrame. iModIntro.
-  iDestruct "clockS" as "[?|clockS]"; last by iRight.
-  iLeft. by iApply Conn.session_failed_failure.
+- iDestruct "Hres" as "(inv & rel)". wp_pures.
+  iApply "post". by iFrame.
 Qed.
 
-Lemma wp_close N c kI kR cs n :
-  {{{ channel c ∗ ctx N ∗ client_connected N kI kR cs n }}}
+Lemma wp_close N c kI kR cs :
+  {{{ channel c ∗ ctx N ∗ client_connected kI kR cs }}}
     close N c (repr cs)
-  {{{ RET #(); client_disconnected N kI kR n ∗ public (si_key cs) }}}.
+  {{{ RET #(); public (si_key cs) }}}.
 Proof.
 iIntros "%Φ (#chan_c & #ctx & conn) post".
-iDestruct "conn" as "(conn & rel & clockC)".
+iDestruct "conn" as "(conn & rel)".
 iPoseProof (Conn.connected_keyE with "conn") as "#(-> & -> & _)".
 wp_lam. wp_pures. wp_list.
 iMod (release with "rel") as "#relC".
@@ -294,10 +248,7 @@ iIntros "conn". wp_pures.
 wp_apply (Conn.wp_read with "[//] [] [$]"); eauto.
 iIntros "%ts (conn & _ & #inv)".
 wp_pures. wp_apply (Conn.wp_free with "[$conn]"). iIntros "_".
-iApply "post". iDestruct "inv" as "[#p_k|[]]".
-iSplit => //. iDestruct "clockC" as "[#comp|clockC]".
-+ iLeft. by iApply Conn.session_failed_failure.
-+ by iRight.
+iApply "post". by iDestruct "inv" as "[#p_k|[]]".
 Qed.
 
 End Proofs.
