rpc/props.v
@@ -44,167 +44,12 @@ Implicit Types v : val.
 Implicit Types (ok : Prop) (failed : bool).
 Implicit Types si : sess_info.
 
-Definition clock k N n :=
-  term_own k N (to_frac_agree (1 / 2) n).
-
-Lemma clock_alloc k N E :
-  ↑N ⊆ E →
-  term_token k E ==∗
-  clock k N 0 ∗
-  clock k N 0 ∗
-  term_token k (E ∖ ↑N).
-Proof.
-iIntros "%sub token".
-iMod (term_own_alloc N (to_frac_agree 1 0) with "token")
-  as "[own token]" => //.
-iFrame. rewrite -Qp.half_half frac_agree_op.
-iDestruct "own" as "[??]". by iFrame.
-Qed.
-
-Lemma clock_agree k N n m :
-  clock k N n -∗
-  clock k N m -∗
-  ⌜n = m⌝.
-Proof.
-iIntros "own1 own2".
-iPoseProof (term_own_valid_2 with "own1 own2") as "%valid".
-rewrite frac_agree_op_valid_L in valid.
-by case: valid.
-Qed.
-
-Lemma clock_update p k N n m :
-  clock k N n -∗
-  clock k N m ==∗
-  clock k N p ∗ clock k N p.
-Proof.
-iIntros "own1 own2". rewrite /clock.
-iMod (term_own_update_2 with "own1 own2") as "[own1 own2]".
-{ apply: (frac_agree_update_2 _ _ _ _ p).
-  by rewrite Qp.half_half. }
-by iFrame.
-Qed.
-
-Variable N : namespace.
-
-Definition never_connected kI kR : iProp :=
-  term_token kR (↑N.@"server".@kI).
-
-Lemma first_connection kI kR :
-  never_connected kI kR ==∗ □ ¬ never_connected kI kR.
-Proof.
-iIntros "token".
-iMod (term_meta_set _ () with "token") as "#meta"; eauto.
-iIntros "!> !> contra".
-by iDestruct (term_meta_token with "contra meta") as "[]".
-Qed.
-
-Definition client_clock kI kR n : iProp :=
-  clock kI (N.@"client".@kR.@"clock".@1) n.
-
-Definition server_clock' kI kR n : iProp :=
-  clock kI (N.@"client".@kR.@"clock".@2) n.
-
-Definition tick kI kR n : iProp :=
-  client_clock kI kR (S n) ∗
-  server_clock' kI kR n ∗
-  (⌜n = 0⌝ ∗ server_clock' kI kR 0 ∨ □ ¬ never_connected kI kR).
-
-Definition tock kI kR n : iProp :=
-  client_clock kI kR n ∗
-  server_clock' kI kR n ∗
-  (⌜n = 0⌝ ∗ server_clock' kI kR 0 ∨ □ ¬ never_connected kI kR).
-
-Definition server_clock kI kR n : iProp :=
-  ⌜n = 0⌝ ∗ never_connected kI kR ∨
-  ⌜n ≠ 0⌝ ∗ server_clock' kI kR n ∗ □ ¬ never_connected kI kR.
-
-Lemma client_clock_tock kI kR n m :
-  client_clock kI kR n -∗
-  tock kI kR m -∗
-  ⌜n = m⌝.
-Proof.
-iIntros "c1 (c2 & _)". iApply (clock_agree with "c1 c2").
-Qed.
-
-Lemma client_clock_alloc kI kR E :
-  ↑N.@"client".@kR.@"clock" ⊆ E →
-  term_token kI E ==∗
-  client_clock kI kR 0 ∗ tock kI kR 0 ∗
-  term_token kI (E ∖ ↑N.@"client".@kR.@"clock").
-Proof.
-iIntros "%sub token".
-iMod (clock_alloc kI ( N:= N.@"client".@kR.@"clock".@1) with "token")
-  as "(? & ? & token)"; first solve_ndisj.
-iFrame.
-iMod (clock_alloc kI ( N:= N.@"client".@kR.@"clock".@2) with "token")
-  as "(c1 & c2 & token)"; first solve_ndisj.
-iModIntro. iFrame.
-iSplitL "c1".
-- iLeft. by iFrame.
-- iApply (term_token_drop with "token"). solve_ndisj.
-Qed.
-
-Lemma server_clock_alloc kI kR E :
-  ↑N.@"server".@kI ⊆ E →
-  term_token kR E ==∗
-  server_clock kI kR 0 ∗ term_token kR (E ∖ ↑N.@"server".@kI).
-Proof.
-iIntros "%sub token".
-rewrite term_token_difference //. iDestruct "token" as "[??]".
-iFrame. iModIntro. iLeft. by iFrame.
-Qed.
-
-Lemma tock_tick kI kR n m :
-  client_clock kI kR n -∗
-  tock kI kR m ==∗
-  ⌜m = n⌝ ∗
-  client_clock kI kR (S n) ∗
-  tick kI kR n.
-Proof.
-iIntros "client1 (client2 & server1 & ?)".
-iPoseProof (clock_agree with "client1 client2") as "<-".
-iFrame.
-iMod (clock_update (S n) with "client1 client2") as "[??]".
-by iFrame.
-Qed.
-
-Lemma tick_tock kI kR n m :
-  server_clock kI kR n -∗
-  tick kI kR m ==∗
-  ⌜m = n⌝ ∗
-  server_clock kI kR (S n) ∗
-  tock kI kR (S n).
-Proof.
-iIntros "server tick".
-iDestruct "server" as "[(-> & never)|(%n0 & s1 & #first1)]";
-iDestruct "tick" as "(c1 & s2 & [(-> & s3)| #first2])".
-- iMod (first_connection with "never") as "#first".
-  iMod (clock_update 1 with "s2 s3") as "[s2 s3]".
-  iModIntro. iSplit => //. iFrame.
-  iSplitL "s2".
-  + iRight. by iSplit; iFrame.
-  + by iRight.
-- by iPoseProof ("first2" with "never") as "[]".
-- iPoseProof (clock_agree with "s1 s2") as "->".
-  iModIntro. by iSplit => //.
-- iPoseProof (clock_agree with "s1 s2") as "<-".
-  iMod (clock_update (S n) with "s1 s2") as "[s1 s2]".
-  iModIntro. iFrame. iSplit => //.
-  iSplitL; last by eauto.
-  iRight. iFrame. by iSplit.
-Qed.
-
-Definition client_disconnected kI kR n : iProp :=
-  Conn.failure kI kR ∨
-  client_clock kI kR n ∗ tock kI kR n.
-
-Definition client_connected kI kR cs n : iProp :=
+Definition client_connected kI kR cs : iProp :=
   Conn.connected kI kR Init cs ∗
-  release_token (si_init_share cs) ∗
-  (compromised_session Init cs ∨ client_clock kI kR n ∗ tock kI kR n).
+  release_token (si_init_share cs).
 
-Lemma client_connected_ok kI kR cs n :
-  client_connected kI kR cs n -∗
+Lemma client_connected_ok kI kR cs :
+  client_connected kI kR cs -∗
   secret kI -∗
   secret kR -∗
   sign_key kI -∗
@@ -215,24 +60,20 @@ iIntros "(conn & _)".
 by iApply (Conn.connected_ok with "conn").
 Qed.
 
-Lemma client_connected_keys kI kR cs n :
-  client_connected kI kR cs n -∗
+Lemma client_connected_keys kI kR cs :
+  client_connected kI kR cs -∗
   ⌜kI = si_init cs⌝ ∗ ⌜kR = si_resp cs⌝.
 Proof.
 iIntros "(conn & _)".
 by iPoseProof (Conn.connected_keyE with "conn") as "(-> & -> & _)".
 Qed.
 
-Definition server_disconnected kI kR n : iProp :=
-  Conn.failure kI kR ∨ server_clock kI kR n.
-
-Definition server_connected kI kR cs n : iProp :=
+Definition server_connected kI kR cs : iProp :=
   Conn.connected kI kR Resp cs ∗
-  release_token (si_resp_share cs) ∗
-  (compromised_session Resp cs ∨ server_clock kI kR n).
+  release_token (si_resp_share cs).
 
-Lemma server_connected_ok kI kR cs n :
-  server_connected kI kR cs n -∗
+Lemma server_connected_ok kI kR cs :
+  server_connected kI kR cs -∗
   secret kI -∗
   secret kR -∗
   sign_key kI -∗
@@ -243,49 +84,19 @@ iIntros "(conn & _)".
 by iApply (Conn.connected_ok with "conn").
 Qed.
 
-Lemma server_connected_keys kI kR cs n :
-  server_connected kI kR cs n -∗
+Lemma server_connected_keys kI kR cs :
+  server_connected kI kR cs -∗
   ⌜kI = si_init cs⌝ ∗ ⌜kR = si_resp cs⌝.
 Proof.
 iIntros "(conn & _)".
 by iPoseProof (Conn.connected_keyE with "conn") as "(-> & -> & _)".
 Qed.
 
-Lemma client_alloc kI kR E :
-  ↑N.@"client".@kR.@"clock" ⊆ E →
-  term_token kI E ={⊤}=∗
-  client_disconnected kI kR 0 ∗
-  term_token kI (E ∖ ↑N.@"client".@kR.@"clock").
-Proof.
-iIntros "%sub kI_token".
-rewrite (term_token_difference _ _ _ sub).
-iDestruct "kI_token" as "[kI_token ?]". iFrame.
-iMod (client_clock_alloc kI (kR := kR)
-       with "kI_token") as "(c1 & c2 & token)" => //.
-iModIntro. iRight. iFrame.
-Qed.
-
-Lemma server_alloc kI kR E :
-  ↑N.@"server".@kI ⊆ E →
-  term_token kR E ==∗
-  server_disconnected kI kR 0 ∗
-  term_token kR (E ∖ ↑N.@"server".@kI).
-Proof.
-iIntros "%sub token".
-rewrite (term_token_difference _ (↑N.@"server".@kI)) //.
-iDestruct "token" as "[token ?]". iFrame.
-iModIntro. iRight. iLeft. by eauto.
-Qed.
-
-Definition call_pred φ kI kR si ts : iProp :=
-  ∃ n, tick kI kR n ∗ φ kI kR si n ts.
-
-Definition resp_pred φ kI kR si ts : iProp :=
-  ∃ n, tock kI kR (S n) ∗ φ kI kR si n ts.
+Variable N : namespace.
 
 Definition rpc_pred (s : string) φ ψ : iProp :=
-  seal_pred (N.@s.@"call") (Conn.conn_pred Init (call_pred φ)) ∗
-  seal_pred (N.@s.@"resp") (Conn.conn_pred Resp (resp_pred ψ)).
+  seal_pred (N.@s.@"call") (Conn.conn_pred Init φ) ∗
+  seal_pred (N.@s.@"resp") (Conn.conn_pred Resp ψ).
 
 Lemma rpc_pred_set (s : string) φ ψ E :
   ↑N.@s ⊆ E →
