store/db.v
@@ -2,9 +2,10 @@ From stdpp Require Import base gmap.
 From mathcomp Require Import ssreflect.
 From stdpp Require Import namespaces coGset.
 From iris.algebra Require Import cmra agree auth csum gset gmap excl frac.
-From iris.algebra Require Import max_prefix_list functions.
+From iris.algebra Require Import functions.
 From iris.heap_lang Require Import notation proofmode.
-From cryptis Require Import lib term gmeta nown cryptis primitives tactics.
+From cryptis Require Import lib term gmeta nown cryptis.
+From cryptis Require Import replica primitives tactics.
 
 Set Implicit Arguments.
 Unset Strict Implicit.
@@ -18,22 +19,17 @@ Variant operation :=
 | Create of term & term
 | Load of term.
 
-Canonical operationO := leibnizO operation.
-
-Definition db_historyUR : ucmra :=
-  authUR (max_prefix_listUR operationO).
-
 Class dbGS Σ := DbGS {
   dbGS_state : inG Σ db_stateUR;
-  dbGS_history : inG Σ db_historyUR;
+  dbGS_replica : replicaG Σ (list operation);
 }.
 
 Local Existing Instance dbGS_state.
-Local Existing Instance dbGS_history.
+Local Existing Instance dbGS_replica.
 
 Definition dbΣ :=
   #[GFunctor db_stateUR;
-    GFunctor db_historyUR].
+    replicaΣ (list operation)].
 
 Global Instance subG_dbGS Σ : subG dbΣ Σ → dbGS Σ.
 Proof. solve_inG. Qed.
@@ -42,8 +38,8 @@ Module DB.
 
 Section DB.
 
-Implicit Types o : operationO.
-Implicit Types os : list operationO.
+Implicit Types o : operation.
+Implicit Types os : list operation.
 Implicit Types db : gmap term term.
 Implicit Types γ : gname.
 Implicit Types N : namespace.
@@ -66,91 +62,6 @@ Definition to_db os : gmap term term :=
   foldl op_app ∅ os.
 
 Context `{!cryptisGS Σ, !heapGS Σ, !dbGS Σ}.
-
-Definition hist_auth k N os : iProp Σ :=
-  term_own k (N.@"hist")
-    (● to_max_prefix_list os ⋅ ◯ to_max_prefix_list os).
-
-Definition db_version k N n : iProp Σ :=
-  ∃ os, ⌜n = length os⌝ ∗ hist_auth k N os.
-
-Definition hist_frag k N os : iProp Σ :=
-  term_own k (N.@"hist")
-    (◯ to_max_prefix_list os).
-
-Local Instance persistent_hist_frag k N os : Persistent (hist_frag k N os).
-Proof. apply _. Qed.
-
-Lemma hist_auth_frag k N os :
-  hist_auth k N os -∗
-  hist_frag k N os.
-Proof. by iIntros "[_ Hown]". Qed.
-
-Lemma hist_frag_agree k N os1 os2 :
-  length os1 = length os2 →
-  hist_frag k N os1 -∗
-  hist_frag k N os2 -∗
-  ⌜os2 = os1⌝.
-Proof.
-move=> lengthE.
-iIntros "#hist1 #hist2".
-iPoseProof (term_own_valid_2 with "hist1 hist2") as "%valid".
-rewrite auth_frag_op_valid to_max_prefix_list_op_valid_L in valid.
-iPureIntro.
-case: valid => - [[|o os] osE].
-- by rewrite app_nil_r in osE.
-- rewrite osE length_app /= in lengthE; lia.
-- by rewrite app_nil_r in osE.
-- rewrite osE length_app /= in lengthE; lia.
-Qed.
-
-Lemma hist_frag_prefix_of os1 os2 k N :
-  os1 `prefix_of` os2 →
-  hist_frag k N os2 -∗
-  hist_frag k N os1.
-Proof.
-iIntros "%os1_os2 #hist_frag". rewrite /hist_frag.
-iApply term_own_mono; last by eauto.
-apply: auth_frag_mono. exact/to_max_prefix_list_included_L.
-Qed.
-
-Lemma hist_update k N os o :
-  hist_auth k N os ==∗
-  hist_auth k N (os ++ [o]) ∗
-  hist_frag k N (os ++ [o]).
-Proof.
-iIntros "auth".
-iMod (term_own_update with "auth") as "auth".
-{ apply: auth_update.
-  apply: (max_prefix_list_local_update os (os ++ [o])).
-  by exists [o]. }
-iDestruct "auth" as "[auth #frag]".
-iModIntro. iSplit => //. by iSplitL.
-Qed.
-
-Definition hist_at k N n os : iProp Σ :=
-  ⌜n = length os⌝ ∗ hist_frag k N os.
-
-Lemma hist_at_agree k N n os1 os2 :
-  hist_at k N n os1 -∗
-  hist_at k N n os2 -∗
-  ⌜os1 = os2⌝.
-Proof.
-iIntros "(-> & #frag1) (%e & #frag2)".
-by iPoseProof (hist_frag_agree with "frag1 frag2") as "->".
-Qed.
-
-Lemma hist_at0 k N os :
-  hist_at k N 0 os -∗
-  ⌜os = []⌝.
-Proof.
-iIntros "(%e_len & #frag)".
-by case: os => [|??] in e_len *.
-Qed.
-
-Definition db_at k N n db : iProp Σ :=
-  ⌜n = 0⌝ ∗ ⌜db = ∅⌝ ∨
-  ∃ os, ⌜db = to_db os⌝ ∗ hist_at k N n os.
 
 Definition to_db_state db : db_stateUR :=
   λ t, ● (Excl' (db !! t)).
@@ -210,25 +121,27 @@ apply: option_local_update.
 by apply: exclusive_local_update.
 Qed.
 
-Definition db_state k N db : iProp Σ :=
-  term_own k (N.@"state") (to_db_state db).
+Implicit Types (kI kR : term).
 
-Definition mapsto k N t1 t2 : iProp Σ :=
-  term_own k (N.@"state") (db_singleton t1 t2).
+Definition db_state kI kR N db : iProp Σ :=
+  term_own kI (N.@"client".@kR.@"state") (to_db_state db).
 
-Definition free_at k N T : iProp Σ :=
-  term_own k (N.@"state") (db_free T).
+Definition mapsto kI kR N t1 t2 : iProp Σ :=
+  term_own kI (N.@"client".@kR.@"state") (db_singleton t1 t2).
 
-Lemma free_at_diff k N T1 T2 :
+Definition free_at kI kR N T : iProp Σ :=
+  term_own kI (N.@"client".@kR.@"state") (db_free T).
+
+Lemma free_at_diff kI kR N T1 T2 :
   T1 ⊆ T2 →
-  free_at k N T2 ⊣⊢ free_at k N T1 ∗ free_at k N (T2 ∖ T1).
+  free_at kI kR N T2 ⊣⊢ free_at kI kR N T1 ∗ free_at kI kR N (T2 ∖ T1).
 Proof.
 move=> sub. by rewrite /free_at db_free_diff // term_own_op.
 Qed.
 
-Lemma db_state_mapsto k N db t1 t2 :
-  db_state k N db -∗
-  mapsto k N t1 t2 -∗
+Lemma db_state_mapsto kI kR N db t1 t2 :
+  db_state kI kR N db -∗
+  mapsto kI kR N t1 t2 -∗
   ⌜db !! t1 = Some t2⌝.
 Proof.
 iIntros "Hauth Hfrag".
@@ -240,11 +153,11 @@ case => incl _.
 by move/Excl_included/leibniz_equiv_iff: incl => <-.
 Qed.
 
-Lemma db_state_update t2' k N db t1 t2 :
-  db_state k N db -∗
-  mapsto k N t1 t2 ==∗
-  db_state k N (<[t1 := t2']>db) ∗
-  mapsto k N t1 t2'.
+Lemma db_state_update t2' kI kR N db t1 t2 :
+  db_state kI kR N db -∗
+  mapsto kI kR N t1 t2 ==∗
+  db_state kI kR N (<[t1 := t2']>db) ∗
+  mapsto kI kR N t1 t2'.
 Proof.
 iIntros "Hauth Hfrag".
 iMod (term_own_update_2 with "Hauth Hfrag") as "own".
@@ -253,11 +166,12 @@ iDestruct "own" as "[Hauth Hfrag]".
 iModIntro. iSplitL "Hauth" => //.
 Qed.
 
-Lemma db_state_create t1 t2 k N db :
-  db_state k N db -∗
-  free_at k N {[t1]} ==∗
-  db_state k N (op_app db (Create t1 t2)) ∗
-  mapsto k N t1 t2.
+Lemma db_state_create t1 t2 kI kR N db :
+  db_state kI kR N db -∗
+  free_at kI kR N {[t1]} ==∗
+  ⌜db !! t1 = None⌝ ∗
+  db_state kI kR N (op_app db (Create t1 t2)) ∗
+  mapsto kI kR N t1 t2.
 Proof.
 iIntros "Hauth Hfree". rewrite /=.
 iAssert (⌜db !! t1 = None⌝)%I as "#->".
@@ -268,232 +182,249 @@ iAssert (⌜db !! t1 = None⌝)%I as "#->".
   by case=> /Excl_included/leibniz_equiv_iff <-. }
 iMod (term_own_update_2 _ _ (a' := (_ ⋅ _)) with "Hauth Hfree") as "[Hauth Hfrag]".
 { by apply: (@db_alloc _ t1 t2). }
-iModIntro. iSplitL "Hauth" => //.
+iModIntro. by iFrame.
 Qed.
 
-Lemma db_state_load t1 k N db :
-  db_state k N db ==∗
-  db_state k N (op_app db (Load t1)).
+Lemma db_state_load t1 kI kR N db :
+  db_state kI kR N db ==∗
+  db_state kI kR N (op_app db (Load t1)).
 Proof. by eauto. Qed.
 
-Definition op_at k N n (o : operation) : iProp Σ :=
-  ∃ os, hist_at k N (S n) (os ++ [o]).
+Definition db_client_ready kI kR N db : iProp Σ :=
+  ∃ os, ⌜db = to_db os⌝ ∗
+        rep_main kI kR N os ∗ rep_current kI kR N [] os.
 
-Lemma op_at_agree k N n o1 o2 :
-  op_at k N n o1 -∗
-  op_at k N n o2 -∗
-  ⌜o1 = o2⌝.
+Definition db_client_waiting kI kR N db o : iProp Σ :=
+  ∃ os, ⌜db = to_db os⌝ ∗
+        rep_main kI kR N (os ++ [o]).
+
+Definition db_server_ready kI kR N db : iProp Σ :=
+  ∃ os, ⌜db = to_db os⌝ ∗ rep_copy kI kR N [] os.
+
+Definition store_call kI kR N t1 t2 : iProp Σ :=
+  ∃ os, rep_update kI kR N [] os (os ++ [Store t1 t2]).
+
+Definition store_resp kI kR N : iProp Σ :=
+  ∃ os, rep_current kI kR N [] os.
+
+Lemma store_callI t1 t2 kI kR N db :
+  db_client_ready kI kR N db ==∗
+  db_client_waiting kI kR N db (Store t1 t2) ∗
+  store_call kI kR N t1 t2.
 Proof.
-iIntros "(%os1 & #hist1) (%os2 & #hist2)".
-iPoseProof (hist_at_agree with "hist1 hist2") as "%e".
-iPureIntro. suff ? : [o1] = [o2] by congruence.
-have e': length os1 = length os2.
-{ move/(f_equal length): e. rewrite !length_app /=. lia. }
-move/(f_equal (drop (length os1))): e.
-by rewrite drop_app_length e' drop_app_length.
+iIntros "(%os & -> & main & cur)".
+iMod (rep_main_update (os ++ [Store t1 t2]) with "main cur")
+  as "[main cur]".
+by iFrame.
 Qed.
 
-Lemma op_at_intro k N n o :
-  db_version k N n ==∗
-  db_version k N (S n) ∗ op_at k N n o.
+Lemma store_callE t1 t2 kI kR N db P :
+  Persistent P →
+  (P ∨ db_server_ready kI kR N db) -∗
+  (P ∨ store_call kI kR N t1 t2) ==∗
+  (P ∨ db_server_ready kI kR N (<[t1 := t2]>db)) ∗
+  (P ∨ store_resp kI kR N).
 Proof.
-iIntros "(%os & -> & auth)".
-iMod (hist_update _ _ _ o with "auth") as "[auth #frag]".
-iModIntro. iSplit.
-- iExists (os ++ [o]). rewrite length_app Nat.add_comm. by iFrame.
-- iExists os. iSplit => //. by rewrite length_app /= Nat.add_comm.
+iIntros "% [#?|(%os & -> & copy)] call".
+{ iModIntro. by iSplitL; eauto. }
+iDestruct "call" as "[#?|(%os' & upd)]".
+{ iModIntro. by iSplitL; eauto. }
+iMod (rep_copy_update with "copy upd") as "(<- & copy & upd)".
+iFrame. iRight. iFrame. by rewrite /to_db foldl_app.
 Qed.
 
-Lemma db_at_op_at k N n db o :
-  db_at k N n db -∗
-  op_at k N n o -∗
-  db_at k N (S n) (op_app db o).
+Lemma store_respE kI kR N db t1 t2 :
+  db_client_waiting kI kR N db (Store t1 t2) -∗
+  store_resp kI kR N -∗
+  db_client_ready kI kR N (<[t1 := t2]>db).
 Proof.
-iIntros "#db_at (%os' & #hist')".
-iAssert (hist_at k N n os') as "hist''".
-{ iDestruct "hist'" as "(%e_n & hist')".
-  rewrite length_app /= in e_n.
-  iSplit; first by iPureIntro; lia.
-  iApply (hist_frag_prefix_of with "hist'").
-  by exists [o]. }
-iDestruct "db_at" as "[[-> ->]|(%os & -> & #hist)]".
-{ iPoseProof (hist_at0 with "hist''") as "->".
-  iRight. iExists [o]. rewrite /to_db /=. by eauto. }
-iPoseProof (hist_at_agree with "hist hist''") as "{hist''} ->".
-iRight. iExists (os' ++ [o]). iSplit => //.
+iIntros "(%os & -> & main) (%os' & cur)".
+iPoseProof (rep_main_current with "main cur") as "<-".
+iFrame. by rewrite /to_db foldl_app.
+Qed.
+
+Definition create_call kI kR N t1 t2 : iProp Σ :=
+  ∃ os, rep_update kI kR N [] os (os ++ [Create t1 t2]) ∗
+        ⌜to_db os !! t1 = None⌝.
+
+Definition create_resp kI kR N : iProp Σ :=
+  ∃ os, rep_current kI kR N [] os.
+
+Lemma create_callI t1 t2 kI kR N db :
+  db !! t1 = None →
+  db_client_ready kI kR N db ==∗
+  db_client_waiting kI kR N db (Create t1 t2) ∗
+  create_call kI kR N t1 t2.
+Proof.
+iIntros "% (%os & -> & main & cur)".
+iMod (rep_main_update (os ++ [Create t1 t2]) with "main cur")
+  as "[main cur]". by iFrame.
+Qed.
+
+Lemma create_callE t1 t2 kI kR N db P :
+  Persistent P →
+  (P ∨ db_server_ready kI kR N db) -∗
+  (P ∨ create_call kI kR N t1 t2) ==∗
+  (P ∨ db_server_ready kI kR N (op_app db (Create t1 t2))) ∗
+  (P ∨ create_resp kI kR N) ∗
+  (P ∨ ⌜db !! t1 = None⌝).
+Proof.
+iIntros "% ready call"; rewrite -!or_sep2.
+iDestruct "ready" as "[?|(%os & -> & copy)]"; eauto.
+iDestruct "call" as "[?|(%os' & upd & %)]"; eauto.
+iMod (rep_copy_update with "copy upd") as "(-> & copy & upd)".
+iModIntro. iRight. iFrame. rewrite /to_db foldl_app. by eauto.
+Qed.
+
+Lemma create_respE kI kR N db t1 t2 :
+  db_client_waiting kI kR N db (Create t1 t2) -∗
+  create_resp kI kR N -∗
+  db_client_ready kI kR N (op_app db (Create t1 t2)).
+Proof.
+iIntros "(%os & -> & main) (%os' & cur)".
+iPoseProof (rep_main_current with "main cur") as "<-". iFrame.
 by rewrite /to_db foldl_app.
 Qed.
 
-Definition store_at k N n t1 t2 : iProp Σ :=
-  op_at k N n (Store t1 t2).
+Definition load_call kI kR N t1 : iProp Σ :=
+  ∃ t2 os, rep_update kI kR N [] os (os ++ [Load t1]) ∗
+           ⌜to_db os !! t1 = Some t2⌝.
 
-Definition create_at k N n t1 t2 : iProp Σ :=
-  op_at k N n (Create t1 t2).
+Definition load_resp kI kR N t2 : iProp Σ :=
+  ∃ t1 os, rep_current kI kR N [] (os ++ [Load t1]) ∗
+           ⌜to_db os !! t1 = Some t2⌝.
 
-Definition load_at k N n t1 :=
-  op_at k N n (Load t1).
+Lemma load_callI t1 t2 kI kR N db :
+  db !! t1 = Some t2 →
+  db_client_ready kI kR N db ==∗
+  db_client_waiting kI kR N db (Load t1) ∗
+  load_call kI kR N t1.
+Proof.
+iIntros "% (%os & -> & main & cur)".
+iMod (rep_main_update (os ++ [Load t1]) with "main cur")
+  as "[main cur]". iFrame. eauto.
+Qed.
 
-Lemma alloc k N E :
-  ↑N ⊆ E →
-  term_token k E ==∗
-  db_version k N 0 ∗
-  db_state k N ∅ ∗
-  free_at k N ⊤ ∗
-  db_at k N 0 ∅ ∗
-  term_token k (E ∖ ↑N).
+Lemma load_callE t1 kI kR N db P :
+  Persistent P →
+  (P ∨ db_server_ready kI kR N db) -∗
+  (P ∨ load_call kI kR N t1) ==∗ ∃ t2,
+  (P ∨ ⌜db !! t1 = Some t2⌝) ∗
+  (P ∨ db_server_ready kI kR N (op_app db (Load t1))) ∗
+  (P ∨ load_resp kI kR N t2).
+Proof.
+iIntros "% ready load".
+iDestruct "ready" as "[?|ready]".
+{ iModIntro. iExists inhabitant. rewrite -!or_sep2. by eauto. }
+iDestruct "load" as "[?|load]".
+{ iModIntro. iExists inhabitant. rewrite -!or_sep2. by eauto. }
+iDestruct "ready" as "(%os & -> & copy)".
+iDestruct "load" as "(%t2 & %os' & upd & %)".
+iMod (rep_copy_update with "copy upd") as "(-> & copy & upd)".
+iModIntro. iExists t2. rewrite -!or_sep2. iRight.
+iFrame. rewrite /to_db foldl_app. by eauto.
+Qed.
+
+Lemma load_respE kI kR N db t1 t2 t2' :
+  db !! t1 = Some t2 →
+  db_client_waiting kI kR N db (Load t1) -∗
+  load_resp kI kR N t2' -∗
+  db_client_ready kI kR N db ∗
+  ⌜t2' = t2⌝.
+Proof.
+iIntros "%db_t1 (%os & -> & main) (%t1' & %os' & cur & %db_t1')".
+iPoseProof (rep_main_current with "main cur") as "%e".
+case: (app_inj_tail _ _ _ _ e) => [<- [<-]] in db_t1' *.
+iFrame. rewrite /to_db foldl_app. iPureIntro.
+split => //. congruence.
+Qed.
+
+Lemma client_alloc kI kR N E :
+  ↑N.@"client".@kR ⊆ E →
+  term_token kI E ==∗
+  db_client_ready kI kR N ∅ ∗
+  db_state kI kR N ∅ ∗
+  free_at kI kR N ⊤ ∗
+  term_token kI (E ∖ ↑N.@"client".@kR).
 Proof.
 iIntros "%sub token".
-iMod (term_own_alloc (N.@"hist")
-        (● to_max_prefix_list [] ⋅ ◯ to_max_prefix_list []) with "token")
-  as "[hist token]"; try solve_ndisj.
-{ apply/auth_both_valid_discrete. split; eauto.
-  exact/to_max_prefix_list_valid. }
-iMod (term_own_alloc (N.@"state") (to_db_state ∅ ⋅ db_free ⊤) with "token")
+iMod (rep_main_alloc (N := N) kI (kR := kR) [] with "token")
+  as "(main & cur & token)"; first solve_ndisj.
+iFrame.
+iMod (term_own_alloc (N.@"client".@kR.@"state")
+        (to_db_state ∅ ⋅ db_free ⊤) with "token")
   as "[[state free] token]"; try solve_ndisj.
 { rewrite /to_db_state /db_free => t /=.
   rewrite discrete_fun_lookup_op lookup_empty /=.
   rewrite -> decide_True; try set_solver.
   rewrite auth_both_valid_discrete Excl_included leibniz_equiv_iff.
   by split. }
-iAssert (hist_at k N 0 []) as "#hist_at".
-{ by iDestruct "hist" as "[??]"; do !iSplit => //. }
-iAssert (db_at k N 0 ∅) as "#db_at".
-{ by iLeft. }
-iAssert (db_version k N 0) with "[hist]" as "auth".
-{ iExists []. by iFrame. }
 iFrame. iModIntro. do !iSplit => //.
 iApply (term_token_drop with "token"). solve_ndisj.
 Qed.
 
-Lemma store_client t2' k N db n t1 t2 :
-  db_version k N n -∗
-  db_at k N n db -∗
-  db_state k N db -∗
-  mapsto k N t1 t2 ==∗
-  db_version k N (S n) ∗
-  db_at k N (S n) (<[t1 := t2']> db) ∗
-  store_at k N n t1 t2' ∗
-  db_state k N (<[t1 := t2']>db) ∗
-  mapsto k N t1 t2'.
+Lemma server_alloc kI kR N E :
+  ↑N.@"server".@kI ⊆ E →
+  term_token kR E ==∗
+  db_server_ready kI kR N ∅ ∗
+  term_token kR (E ∖ ↑N.@"server".@kI).
 Proof.
-iIntros "own_version #db own_db own_frag".
-iMod (op_at_intro _ _ _ (Store t1 t2') with "own_version")
-  as "[own_version #op_at]".
-iPoseProof (db_at_op_at with "db op_at") as "db'".
+iIntros "% token".
+iMod (rep_copy_alloc with "token") as "[??]" => //.
+by iFrame.
+Qed.
+
+Lemma store_client t2' kI kR N db t1 t2 P :
+  Persistent P →
+  (P ∨ db_client_ready kI kR N db) -∗
+  db_state kI kR N db -∗
+  mapsto kI kR N t1 t2 ==∗
+  (P ∨ db_client_waiting kI kR N db (Store t1 t2')) ∗
+  (P ∨ store_call kI kR N t1 t2') ∗
+  db_state kI kR N (<[t1 := t2']>db) ∗
+  mapsto kI kR N t1 t2'.
+Proof.
+iIntros "% ready own_db own_frag".
 iMod (db_state_update t2' with "own_db own_frag") as "[Hstate Hmapsto]".
-iModIntro. iFrame. by iSplit => //.
+iFrame.
+iDestruct "ready" as "[#?|ready]"; first by iModIntro; iSplitL; eauto.
+iMod (store_callI t1 t2' with "ready") as "[??]". by iFrame.
 Qed.
 
-Lemma db_at_store_at k N n db t1 t2 :
-  db_at k N n db -∗
-  store_at k N n t1 t2 -∗
-  db_at k N (S n) (<[t1 := t2]>db).
-Proof. iApply db_at_op_at. Qed.
-
-Lemma create_client t1 t2 k N n db :
-  db_version k N n -∗
-  db_at k N n db -∗
-  db_state k N db -∗
-  free_at k N {[t1]} ==∗
-  create_at k N n t1 t2 ∗
-  db_version k N (S n) ∗
-  db_at k N (S n) (op_app db (Create t1 t2)) ∗
-  db_state k N (op_app db (Create t1 t2)) ∗
-  mapsto k N t1 t2.
+Lemma create_client t1 t2 kI kR N db P :
+  Persistent P →
+  (P ∨ db_client_ready kI kR N db) -∗
+  db_state kI kR N db -∗
+  free_at kI kR N {[t1]} ==∗
+  (P ∨ db_client_waiting kI kR N db (Create t1 t2)) ∗
+  (P ∨ create_call kI kR N t1 t2) ∗
+  db_state kI kR N (op_app db (Create t1 t2)) ∗
+  mapsto kI kR N t1 t2.
 Proof.
-iIntros "version #db_at state Hfree".
-iMod (op_at_intro _ _ _ (Create t1 t2) with "version") as "[version #op_at]".
-iMod (db_state_create t1 t2 with "state Hfree") as "[state mapsto]".
-iModIntro. iFrame. iSplit => //.
-by iApply db_at_op_at.
+iIntros "% ready state Hfree".
+iMod (db_state_create t1 t2 with "state Hfree") as "(%db_t1 & state & mapsto)".
+iFrame.
+iDestruct "ready" as "[#?|ready]".
+{ iModIntro; iSplitL; eauto. }
+iMod (create_callI t2 with "ready") as "[??]" => //. by iFrame.
 Qed.
 
-Lemma db_at_create_at k N n db t1 t2 :
-  db_at k N n db -∗
-  create_at k N n t1 t2 -∗
-  db_at k N (S n) (op_app db (Create t1 t2)).
-Proof. iApply db_at_op_at. Qed.
-
-Lemma load_client t1 k N n db :
-  db_version k N n -∗
-  db_at k N n db ==∗
-  load_at k N n t1 ∗
-  db_version k N (S n) ∗
-  db_at k N (S n) db.
+Lemma load_client t1 t2 kI kR N db P :
+  Persistent P →
+  (P ∨ db_client_ready kI kR N db) -∗
+  db_state kI kR N db -∗
+  mapsto kI kR N t1 t2 ==∗
+  (P ∨ db_client_waiting kI kR N db (Load t1)) ∗
+  (P ∨ load_call kI kR N t1) ∗
+  db_state kI kR N db ∗
+  mapsto kI kR N t1 t2.
 Proof.
-iIntros "version #db".
-iMod (op_at_intro _ _ _ (Load t1) with "version") as "[version #op]".
-iFrame. iModIntro. iSplit=> //. iApply (db_at_op_at with "db op").
-Qed.
-
-Definition stored_at k N n t1 t2 : iProp Σ :=
-  ∃ db, db_at k N n db ∗ ⌜db !! t1 = Some t2⌝.
-
-Lemma load_at_stored_at k N n t1 t2 t1' :
-  stored_at k N n t1 t2 -∗
-  load_at k N n t1' -∗
-  stored_at k N (S n) t1 t2.
-Proof.
-iIntros "(%db & #db & %db_t1) #load".
-iExists db. iSplit => //. iApply (db_at_op_at with "db load").
-Qed.
-
-Lemma db_at0 k N db :
-  db_at k N 0 db -∗
-  ⌜db = ∅⌝.
-Proof.
-iIntros "[[_ ->]|(%os & -> & #hist)]" => //.
-by iPoseProof (hist_at0 with "hist") as "->".
-Qed.
-
-Lemma db_at_agree k N n db1 db2 :
-  db_at k N n db1 -∗
-  db_at k N n db2 -∗
-  ⌜db1 = db2⌝.
-Proof.
-iIntros "#db_at1 #db_at2".
-iPoseProof "db_at1" as "[[-> ->]|db_at1']".
-{ by iPoseProof (db_at0 with "db_at2") as "->". }
-iPoseProof "db_at2" as "[[-> ->]|db_at2']".
-{ by iPoseProof (db_at0 with "db_at1") as "->". }
-iDestruct "db_at1'" as "(%os1 & -> & #hist1)".
-iDestruct "db_at2'" as "(%os2 & -> & #hist2)".
-by iPoseProof (hist_at_agree with "hist1 hist2") as "->".
-Qed.
-
-Lemma db_at_stored_at k N n db t1 t2 :
-  db_at k N n db -∗
-  stored_at k N n t1 t2 -∗
-  ⌜db !! t1 = Some t2⌝.
-Proof.
-iIntros "#db1 (%db' & #db2 & %db_t1)".
-by iPoseProof (db_at_agree with "db1 db2") as "->".
-Qed.
-
-Lemma client_view_stored_at k N n db t1 t2 t2' :
-  db_at k N n db -∗
-  db_state k N db -∗
-  mapsto k N t1 t2 -∗
-  stored_at k N n t1 t2' -∗
-  ⌜t2' = t2⌝.
-Proof.
-iIntros "#db state t1_t2 #stored".
-iPoseProof (db_state_mapsto with "state t1_t2") as "%db_t1".
-iPoseProof (db_at_stored_at with "db stored") as "%db_t1'".
-iPureIntro. rewrite db_t1 in db_t1'. by case: db_t1' => ->.
-Qed.
-
-Lemma stored_atI k N n db t1 t2 :
-  db !! t1 = Some t2 →
-  db_at k N n db -∗
-  stored_at k N n t1 t2.
-Proof. iIntros "%db_t1 #db_at". iExists db; eauto. Qed.
-
-Lemma db_at_to_0 k N n db :
-  db_at k N n db -∗
-  db_at k N 0 ∅.
-Proof.
-iIntros "_". by iLeft.
+iIntros "% ready state mapsto".
+iPoseProof (db_state_mapsto with "state mapsto") as "%db_t1".
+iFrame.
+iDestruct "ready" as "[#?|ready]"; first by iModIntro; iSplitL; eauto.
+iMod (load_callI _ _ _ db_t1 with "ready") as "[??]".
+by iFrame.
 Qed.
 
 End DB.
