replica.v
@@ -1,0 +1,173 @@
+From stdpp Require Import base gmap.
+From mathcomp Require Import ssreflect.
+From stdpp Require Import namespaces coGset.
+From iris.algebra Require Import agree gmap.
+From iris.algebra.lib Require Import dfrac_agree.
+From iris.heap_lang Require Import notation proofmode.
+From cryptis Require Import lib term cryptis.
+
+Set Implicit Arguments.
+Unset Strict Implicit.
+Unset Printing Implicit Defensive.
+
+Notation replicaG Σ A :=
+  (inG Σ (dfrac_agreeR (leibnizO A))).
+
+Notation replicaΣ A :=
+  (GFunctor (dfrac_agreeR (leibnizO A))).
+
+Section Updates.
+
+Context `{!heapGS Σ, !cryptisGS Σ, !replicaG Σ A}.
+
+Implicit Types (kI kR : term) (N : namespace).
+
+Definition replica kI kR N (s : string) (a : A) : iProp Σ :=
+  term_own kI (N.@"client".@kR.@"replica".@s)
+    (to_frac_agree (1 / 2) (a : leibnizO A)).
+
+Lemma replica_alloc kI kR N s a E :
+  ↑N.@"client".@kR.@"replica".@s ⊆ E →
+  term_token kI E ==∗
+  replica kI kR N s a ∗
+  replica kI kR N s a ∗
+  term_token kI (E ∖ ↑N.@"client".@kR.@"replica".@s).
+Proof.
+iIntros "%sub token".
+iMod (term_own_alloc (N.@"client".@kR.@"replica".@s)
+        (to_frac_agree 1 (a : leibnizO A)) with "token")
+  as "[own token]" => //.
+iFrame. rewrite -Qp.half_half frac_agree_op.
+iDestruct "own" as "[??]". by iFrame.
+Qed.
+
+Lemma replica_agree kI kR N s a1 a2 :
+  replica kI kR N s a1 -∗
+  replica kI kR N s a2 -∗
+  ⌜a1 = a2⌝.
+Proof.
+iIntros "own1 own2".
+iPoseProof (term_own_valid_2 with "own1 own2") as "%valid".
+rewrite frac_agree_op_valid_L in valid.
+by case: valid.
+Qed.
+
+Lemma replica_update a kI kR N s a1 a2 :
+  replica kI kR N s a1 -∗
+  replica kI kR N s a2 ==∗
+  replica kI kR N s a ∗ replica kI kR N s a.
+Proof.
+iIntros "own1 own2". rewrite /replica.
+iMod (term_own_update_2 with "own1 own2") as "[own1 own2]".
+{ apply: (frac_agree_update_2 _ _ _ _ (a : leibnizO A)).
+  by rewrite Qp.half_half. }
+by iFrame.
+Qed.
+
+Definition never_connected kI kR N : iProp Σ :=
+  term_token kR (↑N.@"server".@kI).
+
+Lemma first_connection kI kR N :
+  never_connected kI kR N ==∗ □ ¬ never_connected kI kR N.
+Proof.
+iIntros "token".
+iMod (term_meta_set _ () with "token") as "#meta"; eauto.
+iIntros "!> !> contra".
+by iDestruct (term_meta_token with "contra meta") as "[]".
+Qed.
+
+Definition rep_main  kI kR N (a : A) : iProp Σ := replica kI kR N "main" a.
+Definition rep_copy' kI kR N (a : A) : iProp Σ := replica kI kR N "copy" a.
+
+Definition rep_current kI kR N a0 a : iProp Σ :=
+  rep_main  kI kR N a ∗
+  rep_copy' kI kR N a ∗
+  (⌜a = a0⌝ ∗ rep_copy' kI kR N a0 ∨ □ ¬ never_connected kI kR N).
+
+Definition rep_update kI kR N a0 a a' : iProp Σ :=
+  rep_main kI kR N a' ∗
+  rep_copy' kI kR N a ∗
+  (⌜a = a0⌝ ∗ rep_copy' kI kR N a0 ∨ □ ¬ never_connected kI kR N).
+
+Definition rep_copy kI kR N a0 a : iProp Σ :=
+  ⌜a = a0⌝ ∗ never_connected kI kR N ∨
+  rep_copy' kI kR N a ∗ □ ¬ never_connected kI kR N.
+
+Lemma rep_main_current kI kR N a0 a a' :
+  rep_main kI kR N a -∗
+  rep_current kI kR N a0 a' -∗
+  ⌜a = a'⌝.
+Proof.
+iIntros "c1 (c2 & _)". iApply (replica_agree with "c1 c2").
+Qed.
+
+Lemma rep_main_alloc kI kR N a0 E :
+  ↑N.@"client".@kR.@"replica" ⊆ E →
+  term_token kI E ==∗
+  rep_main kI kR N a0 ∗ rep_current kI kR N a0 a0 ∗
+  term_token kI (E ∖ ↑N.@"client".@kR.@"replica").
+Proof.
+iIntros "%sub token".
+iMod (replica_alloc _ a0 (s := "main") with "token")
+  as "(? & ? & token)"; first solve_ndisj.
+iFrame.
+iMod (replica_alloc _ a0 (s := "copy") with "token")
+  as "(c1 & c2 & token)"; first solve_ndisj.
+iModIntro. iFrame.
+iSplitL "c1".
+- iLeft. by iFrame.
+- iApply (term_token_drop with "token"). solve_ndisj.
+Qed.
+
+Lemma rep_copy_alloc kI kR N a0 E :
+  ↑N.@"server".@kI ⊆ E →
+  term_token kR E ==∗
+  rep_copy kI kR N a0 a0 ∗ term_token kR (E ∖ ↑N.@"server".@kI).
+Proof.
+iIntros "%sub token".
+rewrite term_token_difference //. iDestruct "token" as "[??]".
+iFrame. iModIntro. iLeft. by iFrame.
+Qed.
+
+Lemma rep_main_update a' kI kR N a0 a :
+  rep_main kI kR N a -∗
+  rep_current kI kR N a0 a ==∗
+  rep_main kI kR N a' ∗
+  rep_update kI kR N a0 a a'.
+Proof.
+iIntros "client1 (client2 & server1 & ?)".
+iFrame.
+iMod (replica_update a' with "client1 client2") as "[??]".
+by iFrame.
+Qed.
+
+Lemma rep_copy_update kI kR N a0 a1 a2 a' :
+  rep_copy kI kR N a0 a1 -∗
+  rep_update kI kR N a0 a2 a' ==∗
+  ⌜a1 = a2⌝ ∗
+  rep_copy kI kR N a0 a' ∗
+  rep_current kI kR N a0 a'.
+Proof.
+iIntros "server upd".
+iDestruct "server" as "[(-> & never)|(s1 & #first1)]";
+iDestruct "upd" as "(c1 & s2 & [(-> & s3)| #first2])".
+- iMod (first_connection with "never") as "#first".
+  iMod (replica_update a' with "s2 s3") as "[s2 s3]".
+  iModIntro. iSplit => //. iFrame.
+  iSplitL "s2".
+  + iRight. by iSplit; iFrame.
+  + by iRight.
+- by iPoseProof ("first2" with "never") as "[]".
+- iPoseProof (replica_agree with "s1 s2") as "<-".
+  iMod (replica_update a' with "s1 s2") as "[s1 s2]".
+  iModIntro. iFrame. iSplit => //. iSplitL "s1".
+  + by iRight; iFrame.
+  + by iRight.
+- iPoseProof (replica_agree with "s1 s2") as "<-".
+  iMod (replica_update a' with "s1 s2") as "[s1 s2]".
+  iModIntro. iFrame. iSplit => //.
+  iSplitL; last by eauto.
+  iRight. by iFrame.
+Qed.
+
+End Updates.
