store/server_proofs/store.v
@@ -5,7 +5,7 @@ From iris.algebra Require Import agree auth csum gset gmap excl frac.
 From iris.algebra Require Import max_prefix_list.
 From iris.heap_lang Require Import notation proofmode.
 From cryptis Require Import lib term cryptis primitives tactics.
-From cryptis Require Import role conn rpc.
+From cryptis Require Import role iso_dh conn rpc.
 From cryptis.store Require Import impl shared alist db.
 
 Set Implicit Arguments.
@@ -37,27 +37,26 @@ iPoseProof (store_ctx_store with "ctx") as "?".
 iPoseProof (store_ctx_rpc_ctx with "ctx") as "?".
 wp_lam; wp_pures. wp_apply RPC.wp_handle; last by eauto.
 do 3!iSplit => //. clear Φ.
-iIntros "!> %n %ts !> %Φ (#p_ts & #inv_ts & %db & #p_db & db & #db_at) post".
+iIntros "!> %ts !> %Φ (#p_ts & inv_ts & %db & #p_db & db & ready) post".
 wp_pures.
 wp_list_match => [t1 t2 ->|?]; wp_pures; last first.
 { iDestruct "inv_ts" as "[fail|inv_ts]"; last first.
   { by iDestruct "inv_ts" as "(% & % & -> & ?)". }
   wp_list. iApply ("post" $! None). iModIntro. iFrame.
-  rewrite /=. iSplit; eauto. }
+  by rewrite /=. }
 wp_bind (SAList.insert _ _ _).
 iApply (SAList.wp_insert with "db").
 iIntros "!> db". rewrite -fmap_insert.
 wp_pures. wp_list. wp_pures. iApply ("post" $! (Some _)).
+iAssert (compromised_session Resp cs ∨ DB.store_call kI kR N t1 t2)%I
+  with "[inv_ts]" as "inv_ts".
+{ iDestruct "inv_ts" as "[?|(% & % & %e & inv_ts)]"; eauto.
+  case: e => <- <-. by eauto. }
+iMod (DB.store_callE with "ready inv_ts") as "[ready inv_ts]".
 rewrite /=.
-iModIntro. iSplit; first by eauto.
-iFrame.
-iDestruct "p_ts" as "(p_t1 & p_t2 & _)".
-iSplit; first by iApply public_db_insert.
-iDestruct "inv_ts" as "[fail|inv_ts]"; eauto.
-iDestruct "inv_ts" as "(%t1' & %t2' & %e & store_at)".
-case: e => <- <-.
-iDestruct "db_at" as "[fail|db_at]"; eauto.
-iRight. iApply (DB.db_at_store_at with "db_at store_at").
+iModIntro. iFrame. iSplitL; first by eauto.
+iDestruct "p_ts" as "(? & ? & _)".
+by iApply public_db_insert.
 Qed.
 
 End Verif.
